Compute $i[S,H]$:
\begin{dgroup}[]
  \begin{dmath}[]
&i[S,H]=i[-\frac{i\beta}{2mc^2}\mathcal{O},\beta mc^2+\mathcal{O}+\varepsilon]\\
&=\frac{\beta}{2mc^2}[\mathcal{O},\varepsilon]\\
	\end{dmath}
	\begin{dmath}[]
	[\beta\mathcal{O},\mathcal{O}]=\beta\mathcal{O}\mathcal{O}-\mathcal{O}\beta\mathcal{O}
	=2\beta\mathcal{O}^2
	\end{dmath}
	\begin{dmath}[]
	[\mathcal{\beta\mathcal{O},\beta}]=c[\beta\vb{\alpha},\beta]\left(\vb{p}+\frac{e}				{c}\vb{A}\right)=-2\mathcal{O}
	\end{dmath}
\end{dgroup}

\begin{dmath}[]
H'&=\beta mc^2+\frac{\mathcal{O}^2}{2mc^2}-\frac{\mathcal{O}^4}{8m^3c^6}+\mathcal{E}-\frac{[\mathcal{O},[\mathcal{O},\mathcal{E}]]}{8m^2c^4}
\\
-&\frac{i\hbar[\mathcal{O},\mathcal{O}]}{8m^2c^4}+\underbrace{\frac{\beta}{2mc^2}[\mathcal{O},\mathcal{E}]-\frac{\mathcal{O}^3}{2mc^2}+\frac{i\hbar\beta\dot{\mathcal{O}}}{2mc^2}}_{\mathcal{O}'}
\end{dmath}

Repeat $\psi'=e^{-iS'}\psi''$ with $S'=\frac{-i\beta\mathcal{O}'}{2mc^2}$ which leads to
\begin{dmath}[]
H''+H_{\text{even}}+\mathcal{O}''
\end{dmath}
With the third and last iteration
\begin{dmath}[]
\psi''=e^{-iS''}\psi'''\quad S''=\frac{-i\beta\mathcal{O}''}{2mc^2}
\end{dmath}
we arrive at
\begin{dmath}[]
&H'''=H=\beta m c^2+\frac{\mathcal{O}^2}{2mc^2}-\frac{\mathcal{O}^4}{8m^3c^6}+\mathcal{E}\\
&-\frac{[\mathcal{O},[\mathcal{O},\mathcal{E}]]}{8m^2c^4}-\frac{i\hbar[\mathcal{O},\mathcal{O}]}{8m^2c^4}+\mathcal{O}\left(\frac{1}{m^3}\right)\\
\end{dmath}
First term:
\begin{dmath}[]
\frac{\mathcal{O}^2}{2mc^2}&=\frac{1}{2m}\alpha_i(p_i+\frac{e}{c}A_i)\alpha_j(p_j+\frac{e}{c}A_j)\\
&=\frac{1}{2m}\left(\vtr{p}+\frac{e}{c}\vtr{A}\right)^2+\frac{\hbar e}{2m}\vtr{\sigma} \vtr{B} \alpha_i\alpha_j \\
&=\frac{1}{2}\braced{\alpha_i,\alpha_j}+\frac{1}{2}[\alpha_i,\alpha_j]\\
&=\delta_{ij}+i\varepsilon_{ijk}\sigma_k
\end{dmath}
Second term:
\begin{dmath}[]
-\frac{\mathcal{O}^4}{8m^3c^6}=\frac{\vtr p^4}{8m^3c^2}+\ldots\\ (\text{rel. Correction to kinetic Energy})
\end{dmath}

Third term:
\begin{dmath}[]
-\frac{1}{8m^2c^4}[\mathcal{O},[\mathcal{O},\mathcal{E}]]&=\frac{-(-\hbar)^2}{8m^2c^2}\left[\alpha_i\nabla_i
\underbrace{\left[\alpha_j\nabla_j,eV\right]}_{\alpha_je(\nabla_j V-V\nabla_j)=\alpha_je[\nabla_j,V]}\right]\\
&=\frac{(-i\hbar^2)e}{8m^2c^2}\underbrace{\left[\alpha_i\nabla_i,\alpha_jE_j\right]}_{\clubsuit}
\end{dmath}
where
\begin{dmath}[]
\clubsuit &=\alpha_i\alpha_j\nabla_iE_j-\alpha_j\alpha_iE_j\nabla_i\\
&=\nabla\vtr{E}+i\vtr{\sigma}(\nabla\times\vtr{E})-\vtr{E}\cdot\nabla-i\vtr{\sigma}(\vtr{E}\times\nabla)\\
&=[\nabla,\vtr{E}-2i\vtr{\sigma}(\vtr{E}\times\nabla)+i\vtr{\sigma}(\nabla\times\vtr{E})
\end{dmath}

such that we have
\begin{dmath}[]
=\frac{ie\hbar^2}{4m^2c^2}\left(\vtr{\sigma}\cdot(\vtr{E}\times\nabla)-\frac{\vtr{\sigma}(\nabla\times\vtr{E})}{2}\right)-\frac{\hbar^2e}{8m^2c^2}[\nabla\cdot\vtr{E}]
\end{dmath}
ADD MISSING
