\section{The non-relativistic limit}
Consider expansion in $\frac{\vtr{p}}{m}\sim V$ of Dirac equation.

We will derive the Hamiltionian used in section 2 (for fine structure)

Dirac equation in presence of em field: 
\begin{dgroup}[]
	\begin{dmath}[]
		p^{\nu}\to p^{\nu}+\frac{e}{c}A^{\nu}
	\end{dmath}
	\begin{dsuspend}
		write
	\end{dsuspend}
	\begin{dmath}[]
		\psi=
		\begin{pmatrix}
			\chi\\
			\eta
		\end{pmatrix}
		\condition{2-componenent-spinors}
	\end{dmath}
	\begin{dmath}[]
		\cancel{p}+\frac{e}{c}\cancel{A}-mc
	\end{dmath}
	\begin{dmath}[]
		\begin{pmatrix}
			\chi\\
			\eta
		\end{pmatrix}
		=
		\begin{pmatrix}
			\frac{E}{c}+\frac{e}{c}\phi-mc&-\left( \vtr{p}+\frac{e}{c}\vtr{A} \right)\cdot \vtr{\upsigma}\\
			\left( \vtr{p}+\frac{e}{c}\vtr{A} \right)\cdot \vtr{\upsigma}& -\left( \frac{E}{c}+\frac{e}{c}\phi+mc \right)
		\end{pmatrix}
		\begin{pmatrix}
			\chi\\
			\eta
		\end{pmatrix}
		=0
	\end{dmath}
	\begin{dmath}[label=eq:starnonrellim]
		\hiderel{\Rightarrow} 
		\left( \frac{E}{c}+\frac{e}{c}\phi -mc \right)\chi
		=\left( \vtr{p}+\frac{e}{c}\vtr{A} \right)\cdot \vtr{\upsigma} \eta
	\end{dmath}
	\begin{dmath}[]
		\left( \vtr{p}+\frac{e}{c}\vtr{A} \right)\cdot \vtr{\upsigma} \chi
		=\left( \frac{E}{c}+mc+\frac{e}{c}\phi \right)\eta
	\end{dmath}
	\begin{dmath}[label=eq:trianglenonrellim]
		\hiderel{\leadsto} \eta=\frac{\left( \vtr{p}+\frac{e}{c}\vtr{A} \right)\cdot \vtr{\upsigma}}{\frac{E}{c}+mc+\frac{e}{c}\phi}\chi
		\approx \frac{\left( \vtr{p}+\frac{e}{c}\vtr{A} \right)\cdot \upsigma}{2mc}\chi
	\end{dmath}
	\begin{dsuspend}
		Putting Eq. \ref{eq:trianglenonrellim} in Eq. \ref{eq:starnonrellim} gives us
	\end{dsuspend}
	\begin{dmath}[]
		\left( \frac{E}{c}+\frac{e}{c}\phi-mc \right)\chi
		=\left( \vtr{p}+\frac{e}{c}\vtr{A} \right)\cdot \vtr{\upsigma} \left( \vtr{p}+\frac{e}{c}\vtr{A} \right)\cdot \vtr{\upsigma} \frac{1}{2mc}\chi
		=\frac{1}{2mc}\left( \left( \vtr{p}+\frac{e}{c}\vtr{A} \right)^2 +i\left( -i\hbar \right)\frac{e}{c}\underbrace{\left( \vtr{\nabla}\times \vtr{A}+\vtr{A}\times\vtr{\nabla} \right)}_{\left[ \nabla\times \vtr{A} \right]}\cdot \vtr{\upsigma} \right)\chi
	\end{dmath}
	\begin{dsuspend}
		``derivative within $\left[ \cdot \right]$ only''
	\end{dsuspend}
	\begin{dmath}[]
		\hiderel{\Rightarrow}
		\left( \frac{1}{2m}\left( \vtr{p}\cdot \frac{e}{c}\vtr{A} \right)^2 +\frac{\hbar e}{2mc}\vtr{\upsigma} \cdot \vtr{B}-e\phi \right)\chi
		=\left( E-mc^2 \right)\chi=\hiderel{:}E' \chi
	\end{dmath}
	\begin{dsuspend}
		where $\frac{\hbar e}{2mc}\vtr{\upsigma} \cdot \vtr{B}$ has to be compare to section 2.3 with
	\end{dsuspend}
	\begin{dmath}[]
		H\sim \vtr{\upmu}\cdot \vtr{B}
		=\frac{e}{2m} g \vtr{S}\cdot \vtr{B}
		=\frac{e}{4m}g\vtr{\upsigma}\cdot \vtr{B}
	\end{dmath}
	\begin{dmath}[]
		\hiderel{\Rightarrow} g=2
	\end{dmath}
\end{dgroup}
Let's do this more systematically (expand in $\frac{\abs{e}}{m}$)

Find transformation
\begin{dgroup}[]
	\begin{dmath}[]
		\psi=e^{-iS}\psi'\condition{(Foldy-Wontthuysen transformation)}
	\end{dmath}
	\begin{dsuspend}
		such thath odd operators are suppressed by $\left( \frac{\abs{p}}{m} \right)^n$ $\leadsto$ mixes $\chi$ and $\eta$
	\end{dsuspend}
	\begin{dmath}[]
		\sigma\hiderel{:}=c\vtr{\upalpha}\left( \vtr{p}+\frac{e}{c}\vtr{A} \right)
	\end{dmath}
	\begin{dmath}[]
		i\hbar\partial_t\psi'=i\hbar\partial_te^{iS}\psi
		=i\hbar \left[ \partial_{t}e^{iS} \right]\psi +e^{@S}i\hbar\partial_{t}\psi
		=i\hbar \left[ \partial_{t}e^{+iS} \right]e^{-iS}\psi'+e^{iS}He^{-iS}\psi'
		=\hiderel{:}H'\psi'
	\end{dmath}
	\begin{dmath}[]
		H'=H+i\comm{S}{H}+\frac{i^2}{2!}\comm{S}{\comm{S}{H}}+\frac{i^3}{3!}\ldots
		-\hbar \dot{S}-\frac{i\hbar}{2!}\comm{S}{\dot{S}}-\frac{i^2\hbar}{3!}\comm{S}{\comm{S}{\dot{S}}}\ldots
	\end{dmath}
	\begin{dsuspend}
		Recall
	\end{dsuspend}
	\begin{dmath}[]
		H=\beta mc^2 +\sigma +\xi\condition{even: $\xi=-e\phi$}
	\end{dmath}
	\begin{dsuspend}
		Set
	\end{dsuspend}
	\begin{dmath}[]
		S=\frac{-i\beta}{2mc^2}\sigma
	\end{dmath}
	\begin{dsuspend}
		Compute
	\end{dsuspend}
	\begin{dmath}[]
		i\comm{S}{H}=i\comm{\frac{-i\beta}{2mc^2}\sigma}{\beta mc^2+\sigma+\xi}
		=\frac{\beta}{2mc^2}\comm{\sigma}{\xi}+\frac{\beta}{mc^2}\sigma^2 -\sigma
	\end{dmath}
\end{dgroup}
