\chapter{General scattering theory}
General scattering more complicated than in section 6 e.g. production of new particles. Want to use general representation, so $\ket{\psi}$ is a general state in Hilbert space (not nec. wave function)
\section{Dynamics of scattering}
Start from time dependent Schrödinger
\begin{dgroup}[]
	\begin{dmath}[]
		i\hbar\partial_{t}\ket{\psi,t}=H\ket{\psi,t}
	\end{dmath}
	\begin{dmath}[]
	H=H_0+V
	\end{dmath}
	\begin{dmath}[]
		\ldots = \ldots
	\end{dmath}
	\begin{dmath}[]
		\left( i\hbar \partial_t-H_0 \right)\ket{\psi,t}=V\ket{\psi,t}=\ket{\chi,t}
	\end{dmath}
\end{dgroup}
\begin{defn}
	Green operation $G_0\left( t,t' \right)$ through
	\begin{dmath}[]
	\left( i\hbar \partial_t-H_0 \right)G_0\left( t,t' \right)=
	\delta\left( t-t' \right)\cdot \vtr{1}\condition{($\leftarrow$ operators)}
	\end{dmath}
	inhomogeneous differential equation in $t$
\end{defn}
\paragraph{solutions}
\begin{dgroup}[]
	\begin{dmath}[]
		G_{0}^{+}\left( t,t' \right)=-\frac{i}{\hbar}\theta\left( t-t' \right)e^{-\frac{i}{\hbar}H_0\left( t-t' \right)}
	\end{dmath}
	\begin{dmath}[]
		G_{0}^{-}\left( t,t' \right)=+\frac{i}{\hbar}
	\end{dmath}
\end{dgroup}

\begin{proof}
	\begin{dgroup}[]
		\begin{dmath}[]
			i\hbar\partial_tG_{0}^{+}\left( t-t' \right)=i\hbar\left( -\frac{i}{\hbar} \right)\partial_t\theta\left( t-t' \right)e^{-\frac{i}{\hbar}H_0\left( t-t' \right)}
			=\delta\left( t-t' \right)e^{-\frac{i}{\hbar}H_0\left( t-t' \right)}+\theta\left( t-t' \right)\left( -\frac{i}{\hbar}H_0 \right)e^{-\frac{i}{\hbar}H_0\left( t-t' \right)}
			=\delta\left( t-t' \right)+H_0G_{0}^{+}\left( t-t' \right)
		\end{dmath}
	\end{dgroup}
	Note: The superscripts $\pm$ are related to those in section 6
	\begin{dgroup}[]
		\begin{dmath}[]
			G_{0}^{\pm}\left( t,t' \right)=G_{0}^{pm}\left( t-t' \right)
		\end{dmath}
		\begin{dsuspend}
			Write solution to Schrödinger
		\end{dsuspend}
		\begin{dmath}[]
			\ket{\psi^{\pm},t}=\ket{\psi^0,t}+\int_{}^{}\dd{t'}G_{0}^{\pm} \left( t-t' \right)V\ket{\psi^{\pm},t'}
		\end{dmath}
		\begin{dsuspend}
			with $\ket{\psi^{0},t}$ solution to homogeneous problem
		\end{dsuspend}
		\begin{dmath}[]
			\left( i\hbar\partial_t-H_{0} \right)\ket{\psi_0,t}=0
		\end{dmath}
	\end{dgroup}
	The ``physical'' solution is given by $\ket{\psi^{+},t}$, since $G^{+}\left( t-t' \right)$ moves ``forward'' in time. (retardation)

	To make connection with section 6: $t\to E$
	\begin{dgroup}[]
		\begin{dmath}[]
			G_{0}^{+}\left( E \right)=\int_{-\infty}^{\infty}\dd{t}\, e^{\frac{i}{\hbar} Et}G_{0}^{+}(t)
			=-\frac{i}{\hbar}\int_{0}^{\infty}\dd{t}\, e^{\frac{i}{\hbar}Et}e^{-\frac{i}{\hbar}H_0t}
		\end{dmath}
		\begin{dsuspend}
			with
		\end{dsuspend}
		\begin{dmath}[]
			G_{0}^{+}(t)=G_{0}^{+}\left( t,t'\hiderel{=}0 \right)
		\end{dmath}
		\begin{dsuspend}
			for $t\to \infty$ need $E\to E+i0^{+}, 0^{+}>0$
		\end{dsuspend}
		\begin{dmath}[]
			G_{0}^{\pm}=\frac{1}{E-H_0\pm i0^{+}}
			\equiv \left( E-H_0\pm i0^{+} \right)^{-1}
		\end{dmath}
	\end{dgroup}
\end{proof}
$\ket{\psi^{\pm},t}$ evolves with $H$, but was equal to free state $\ket{\psi^{0},t}$ @ $t\to-\infty$

Let $\alpha$ be a complete set of quantum number of $H_0$ (including $E_{\alpha}$)
\begin{dgroup}[]
	\begin{dmath}[]
		\hiderel{\to} \ket{\psi_{\alpha}^{0},t}\leftrightarrow \ket{\psi_{\alpha}^{\pm},t}
	\end{dmath}
	\begin{dsuspend}
		make Fourier $t\to E$ of Eq. $\pm$
	\end{dsuspend}
	\begin{dmath}[]
		\underbrace{\int_{}^{}\dd{t}\, e^{\frac{i}{\hbar}Et}\ket{\psi_{\alpha}^{\pm},t}}_{\ket{\psi_{\alpha}^{\pm}(E)}\to \ket{\psi_{\alpha}^{\pm}}}=\underbrace{\int_{}^{}\dd{t}\, e^{\frac{i}{\hbar}Et}\ket{\psi_{\alpha}^{0},t}}_{\ket{\psi_{\alpha}^{0}\left( E \right)}\sim \ket{\psi_{\alpha}^{0}}}
		+\int_{}^{}\dd{t}\, e^{\frac{i}{\hbar}Et}\underbrace{\int_{}^{}\dd{t'}\, G_{0}^{\pm}\left( t-t' \right)}_{t\to t+t'}V\ket{\psi_{\alpha}^{\pm},t}
	\end{dmath}
	\begin{dmath}[]
		\int_{}^{}\dd{t}\, e^{\frac{i}{\hbar}Et}G_{0}^{+}(t)=G_{0}^{+}(E)
	\end{dmath}
	\begin{dmath}[]
		V\ket{\psi_{\alpha}^{\pm}(E)}=\int_{}^{}\dd{t'} \, e^{\frac{i}{\hbar}Et'}V\left( \psi_{\alpha}^{\pm}(E) \right)
	\end{dmath}
\end{dgroup}
\begin{dgroup}[]
	\begin{dmath}[]
		\ket{_{\alpha}^{\pm}}=\ket{\psi_{\alpha}^{0}}+G_{0}^{\pm}V\ket{\psi_{\alpha}^{\pm}}\condition{(Lippmann-Schwinger)}
	\end{dmath}
\end{dgroup}
Solution:
\begin{dgroup}[]
	\begin{dmath}[]
		\ket{\psi_{\alpha}^{\pm}}=\left( 1-G_{0}^{\pm}V \right)^{-1}\ket{\psi_{\alpha}^{0}}
		=\frac{1}{\left( G_{0}^{\pm} \right)^{-1}-V}\left( G_{0}^{pm} \right)^{-1}\ket{\psi_{\alpha}^{0}}
		=\frac{1}{E_{\alpha}-H_0\pm i0^{+}-V}\left( E_{`?a}-H_0\pm i0^{+}-V+V \right)\ket{\psi_{\alpha}^{0}}
		=\underbrace{\frac{1}{E_{\alpha}-H\pm i0^{+}}}_{G^{\pm}E_{\alpha}}\left( E_{\alpha}-H+V\pm i0^{+} \right)\ket{\psi_{\alpha}^{0}}
		=\left( 1+G^{\pm}V \right)\ket{\psi_{\alpha}^{0}}
	\end{dmath}
	\begin{dmath}[]
		\psi_{\alpha}^{\pm}=\left( 1+G^{\pm}V \right)\ket{\psi_{\alpha}^{0}}
	\end{dmath}
	\begin{dsuspend}
		can also be obtained from (exercise 2)
	\end{dsuspend}
	\begin{dmath}[]
		\ket{\psi^{\pm},t}=\lim_{t'\to \mp \infty}i\hbar G^{+}\left( t-t' \right)\ket{\psi_0,t'}
	\end{dmath}
\end{dgroup}
\section{M\o ller operators \& scattering operator}
$\alpha$: Complete set of quantum numbers
\begin{dgroup}[]
	\begin{dmath}[]
		H_0\ket{\psi_{\alpha}^{0}}=E_{\alpha}\ket{\psi_{\alpha}^{0}}
	\end{dmath}
	\begin{dmath}[]
		H\ket{\psi_{\alpha}^{\pm}}=E_{\alpha}\ket{\psi_{\alpha}^{\pm}}
	\end{dmath}
	\begin{dsuspend}
		Consider again
	\end{dsuspend}
	\begin{dmath}[]
		\ket{\psi_{\alpha}^{\pm}}=\ket{\psi_{\alpha}^{0}}+\left( E_{\alpha}-H_0+\pm O^{+} \right)^{-1}V\ket{\psi_{\alpha}^{\pm}}
		=\ket{\psi_{\alpha}^{0}}+\int_{}^{}\dd{\beta}\, \frac{T_{\beta\alpha}\ket{\psi_{\beta}^{0}}}{E_{\alpha}-E_{\beta}\pm i0^{+}}
	\end{dmath}
	\begin{dmath}[]
		1=\int_{}^{}\dd{\beta}\, \proj{\psi_{\beta}^{0}}
	\end{dmath}
	\begin{dmath}[]
		T_{\beta\alpha}\equiv \mel{\psi_{\beta}^{0}}{V}{\psi_{\alpha}^{\pm}}
	\end{dmath}
	\begin{dsuspend}
		Transfer matrix
	\end{dsuspend}
\end{dgroup}
This state satisfies:
\begin{dgroup}[]
	\begin{dmath}[]
		\int_{}^{}\dd{\alpha}\, e^{-\frac{i}{\hbar}E_{\alpha}\tau}f(\alpha)\ket{\psi_{\alpha}^{\pm}}
		\xrightarrow{\tau\to \mp \infty}\int_{}^{}\dd{\alpha} \, e^{-\frac{i}{\hbar}E_{\alpha}\tau}f(\alpha)\ket{\psi_{\alpha}^{0}}
	\end{dmath}
	\begin{dsuspend}
		or
	\end{dsuspend}
	\begin{dmath}[]
		e^{-\frac{i}{\hbar}H\tau}\int_{}^{}\dd{\alpha}\, f(\alpha)\ket{\psi_{\alpha}^{\pm}}\xrightarrow{e^{-\frac{i}{\hbar}H_0\tau}}\int_{}^{}\dd{\alpha}\, f(\alpha)\ket{\psi_{\alpha}^{0}}
	\end{dmath}
	\begin{dmath}[]
		\hiderel{\Rightarrow}\ket{\psi_{\alpha}^{\pm}}=\lim_{\tau\mp \infty}e^{+\frac{i}{\hbar}H\tau}e^{-\frac{i}{\hbar}H_0\tau}\ket{\psi_{\alpha}^{0}}=\Omega^{\pm}\ket{\psi_{\alpha}^{0}}
	\end{dmath}
	\begin{dsuspend}
		with $\Omega^{\pm}$ M\o ller operators
	\end{dsuspend}
\end{dgroup}
\emph{Typical} scattering experiment:

At $t\to -\infty$ prepare state with quantum number $\alpha$ of $H_0$

Q: What is amplitude for this state to end up in (another) eigenstate of $H_0$ with quantum number $\beta$.

A: 
%\begin{dgroup}[]
	\begin{dmath}[]
		\braket{\psi_{\beta}^{-}}{\psi_{\alpha}^{+}}=\mel{\psi_{\beta}^{0}}{\left( \Omega^{-} \right)^{\dagger}\Omega^{+}}{\psi_{\alpha}^{0}}
		\equiv \mel{\psi_{\beta}^{0}}{S}{\psi_{\alpha}^{0}}
	\end{dmath}
%\end{dgroup}
\begin{dsuspend}
		$S=$Scattering operator, with
	\end{dsuspend}
	\begin{dmath}[]
		S=\lim_{\substack{\tau\to \infty\\ \tau\to -\infty}}e^{\frac{i}{\hbar}H_0\tau}e^{\frac{i}{\hbar}H\left( \tau_0-\tau \right)}e^{-\frac{i}{\hbar}H_0\tau_0}
		=\lim_{\substack{\tau\to\infty\\ \tau_0\to -\infty}}U\left( \tau,\tau_0 \right)=U\left( \infty,-\infty \right)
\end{dmath}
ex 1: sheet 6:
\begin{dgroup}[]
	\begin{dmath}[]
		i\hbar\dv{}{\tau}U\left( \tau,\tau_0 \right)=e^{\frac{i}{\hbar}H_0\tau}\left( H-H_0 \right)e^{\frac{i}{\hbar}H\left( \tau_0-\tau \right)}e^{-\frac{i}{\hbar}H_0\tau_0}
		=\underbrace{e^{\frac{i}{\hbar}H_0\tau}Ve^{-\frac{i}{\hbar}H_0\tau}}_{V(\tau)}U\left( \tau,\tau_0 \right)
		=V(\tau)U\left( \tau,\tau_0 \right)
	\end{dmath}
\end{dgroup}
$V(\tau)$ evolution operator in IA picture section 4.4. Solution
\begin{dgroup}[]
	\begin{dmath}[]
		U\left( \tau,\tau_0 \right)=T\left( e^{-\frac{i}{\hbar}\int_{\tau_0}^{\tau}\! V(\tau)\dd{\tau}} \right)
	\end{dmath}
	\begin{dsuspend}
		and
	\end{dsuspend}
	\begin{dmath}[]
		S=U\left( \infty,-\infty \right)
		=\vtr{1}-\frac{i}{\hbar}\int_{-\infty}^{\infty}\! \dd{t_1}V(t_1)+\left( -\frac{i}{\hbar} \right)^{2}\int_{-\infty}^{\infty}\! \dd{t_1}\int_{-\infty}^{t_1}\! \dd{t_2}V(t_1)V(t_2)+\ldots
	\end{dmath}
\end{dgroup}
Note:
\begin{dmath}[]
	SS^{\dagger}=\vtr{1}\condition{$S$ operator is unitary}
\end{dmath}
$S$-matrix 
\begin{dmath}[]
	S_{\beta\alpha}\equiv \mel{\psi_{\beta}^{0}}{S}{\psi_{\alpha}^{0}}
	=\braket{\psi_{\beta}^{-}}{\psi_{\alpha}^{\dagger}}
\end{dmath}
\paragraph{option 1} insert $S$ operator
\begin{description}
	\item[1st term:]
		\begin{dmath}[]
			\mel{\psi_{\beta}^{0}}{\vtr{1}}{\psi_{\alpha}^{0}}=\delta\left( \beta-\alpha \right)
		\end{dmath}
	\item[2nd term] 
		\begin{dmath}[]
			-\frac{i}{\hbar}\int_{-\infty}^{\infty}\! \dd{t_1}\mel{\psi_{\beta}^{0}}{e^{\frac{i}{\hbar}H_0t}Ve^{-\frac{i}{\hbar}H_0t}}{\psi_{\alpha}^{0}}
			=-\frac{i}{\hbar}\int_{}^{}\dd{t}e^{-\frac{i}{\hbar}\left( E_{\alpha}-E_{\beta} \right)t}\mel{\psi_{\beta}^{0}}{V}{\psi_{\alpha}^{0}}
			=-2i\pi \delta\left( E_{\alpha}-E_{\beta} \right)V_{\beta\alpha}
		\end{dmath}
	\item[3rd and 4th] $\to$ exercise sheet 8
\end{description}
