\section{Quantization of relativistic fields}
\begin{itemize}
	\item Start with Lagrangian density $\mathcal{L}$ for classical field tehory
	\item Compute conjugate momentum field
	\item impose equal-time (anti-) commutation relations
\end{itemize}
\paragraph{Example 1: free scalar field $\Phi(\vtr{x},t)=\Phi(x)$}
\begin{itemize}
	\item 
		\begin{dgroup}[]
			\begin{dmath}[]
				\mathcal{L}=\frac{1}{2}\partial_{\mu}\Phi\partial^{\mu}\Phi-\frac{1}{2}\underbrace{\frac{m^2c^2}{\hbar^2}}_{\equiv m^2}\Phi^2-\underbrace{V(\Phi)}_{=0}
			\end{dmath}
			\begin{dsuspend}
				free field (no interactions). Action:
			\end{dsuspend}
			\begin{dmath}[]
				S=\int_{}^{}\dd{t}\int_{}^{}\rd^3 x\, \mathcal{L}
				=\int_{}^{}\rd^3 4 x \, \mathcal{L}\left( \Phi, \partial_{\mu}\Phi \right)
			\end{dmath}
			\begin{dmath}[]
				\delta S=0
			\end{dmath}
			\begin{dmath}[]
				\hiderel{\to} \pdv{\mathcal{L}}{\Phi}-\partial_{\mu}\pdv{\mathcal{L}}{\left( \partial_{\mu}\Phi \right)}90
			\end{dmath}
			\begin{dsuspend}
				for our $\mathcal{L}$:
			\end{dsuspend}
			\begin{dmath}[]
				-m^2\Phi-\partial_{\mu}\partial^{\mu}\Phi=0
			\end{dmath}
			\begin{dsuspend}
				Klein-Gordan equation
			\end{dsuspend}
		\end{dgroup}
	\item Conjugate momentum field
		\begin{dgroup}[]
			\begin{dmath}[]
				\pi\left( \vtr{x},t \right)=\pdv{\mathcal{L}}{\Phi}=\dot{\phi}\left( \vtr{x},t \right)
			\end{dmath}
			\begin{dsuspend}
				Hamiltonian
			\end{dsuspend}
			\begin{dmath}[]
				H=\int_{}^{}\rd^3 \vtr{x}\, \pi\dot{\Phi}-L
				=\int_{}^{}\rd^3 x\, \left( \pi\dot{\phi}-\mathcal{L} \right)
				=\frac{1}{2}\int_{}^{}\rd^3 x\, \left( \pi^2 +\left( \nabla \Phi \right)^2+m^2\Phi^2 \right)
			\end{dmath}
			\begin{dsuspend}
				with $\mathcal{L}$ the Lagrangian density 
			\end{dsuspend}
			\begin{dmath}[]
				\int_{}^{}\rd^3 x\, \mathcal{L}=L=\text{Lagriangian}
			\end{dmath}
		\end{dgroup}
	\item 
		now second quantization:
		\begin{dgroup}[]
			\begin{dmath}[]
				\Phi(x)\to \hat{\Phi(x)}
			\end{dmath}
			\begin{dsuspend}
				and
			\end{dsuspend}
			\begin{dmath}[]
				\pi (x)\to \hat{\pi}(x)
			\end{dmath}
			\begin{dmath}[]
				\comm{\hat{\phi}\left( \vtr{x},t \right)}{\hat{\phi}\left( \vtr{y},t \right)}
				=\comm{\hat{\pi}\left( \vtr{x},t \right)}{\hat{\pi}\left( \vtr{y},t \right)}=0
			\end{dmath}
			\begin{dsuspend}
				impose
			\end{dsuspend}
			\begin{dmath}[]
				\comm{\hat{\Phi}\left( \vtr{x},t \right)}{\hat{\pi}\left( \vtr{y},t \right)}
				=i\delta\left( \vtr{x}-\vtr{y}\right)
			\end{dmath}
			\begin{dmath}[]
				\hiderel{\sim} \comm{x_i}{p_j}=i\delta_{ij}\condition*{\left( \hbar=1 \right)}
			\end{dmath}
			\begin{dsuspend}
				spin $0$, bosonic field use $\comm{\cdot}{\cdot}=\comm{\cdot}{\cdot}_{-}$ and not $\acomm{\cdot}{\cdot}=\comm{\cdot}{\cdot}_{+}$
			\end{dsuspend}
			\begin{dsuspend}
				now as for radiation field
			\end{dsuspend}
			\begin{dmath}[]
				\hat{\Phi}\left( \vtr{x},t \right)=\int_{}^{}\frac{\rd^3 k}{\left( 2\pi \right)^{3}}\frac{1}{2\omega_k}\left( \hat{a}_{k}e^{i\vtr{k}\vtr{x}-i\omega_{k}t}+\hat{a}_{k}^{\dagger}e^{-i\vtr{k}\vtr{x}+i\omega_{k}t} \right)
			\end{dmath}
			\begin{dsuspend}
				with $\omega_k=\sqrt{\vtr{k}^2+m^2}$ this satisfies KGE
			\end{dsuspend}
			\begin{dmath}[]
				\hat{\pi}\left( \vtr{x},t \right)=\dot{\hat{\Phi}}\left( \vtr{x},t \right)
				=\int_{}^{}\frac{\rd^3 k}{\left( 2\pi \right)^3}\frac{1}{2\omega_k}\left( -i\omega_{k}\hat{a}_ke^{i\vtr{k}\vtr{x}-i\omega_k t}+i\omega_k\hat{a}_{k}^{\dagger}e^{-i\vtr{k}\vtr{x}+i\omega_k t} \right)
			\end{dmath}
			\begin{dsuspend}
				Note: change in normalization:
			\end{dsuspend}
			\begin{dmath}[]
				\int_{}^{}\frac{\rd^3 \vtr{k}}{\left( 2\pi \right)^3}\hiderel{\to}\underbrace{\int_{}^{}\frac{\rd^3 \vtr{k}}{\left( 2\pi \right)^3 }\frac{1}{2\omega_k}}_{\mathclap{\text{Lorentz invariant}}}
			\end{dmath}
		\end{dgroup}
\end{itemize}
\begin{proof}
	\begin{dgroup}[]
		\begin{dmath}[]
			\int_{}^{}\frac{\rd^3 k}{\left( 2\pi \right)^4}2\pi \delta\left( k^2-m^2 \right)\sigma(k_0) \condition{(manifestly $L$-invariant)}
			=\int_{}^{}\frac{\rd^4 k}{\left( 2\pi \right)^3}\delta\left( k^2-m^2 \right)\vartheta\left( k_0 \right)
			=\int_{}^{}\frac{\rd^4 k}{\left( 2\pi \right)^3} \frac{1}{2\omega_k}\left( \delta\left( k_0-\omega_k \right)+\delta\left( k_0+\omega_k \right)\vartheta\left( k_0 \right) \right)
			=\int_{}^{}\frac{\rd^3 \vtr{k}}{\left( 2\pi \right)^3}\frac{1}{\omega_k}
		\end{dmath}
		\begin{dsuspend}
			where in $\delta\left( k_0+\omega_k \right)$ $\omega_k$ does not contribute and we used
		\end{dsuspend}
		\begin{dmath}[]
			\delta\left( f(x) \right)=\sum_{i}^{}\frac{1}{\abs{f(x_i)}}\delta(x_i)\condition*{f(x_i)=0}
		\end{dmath}
		\begin{dsuspend}
			Express $\hat{a}_k$ and $\hat{a}_{k}^{\dagger}$ in terms of $\hat{\phi}$ and $\hat{\pi}$
		\end{dsuspend}
		\begin{dmath}[]
			\int_{}^{}\rd^3 x\, e^{i\vtr{k}\cdot \vtr{x}}\left( \omega_k\hat{\phi}(\vtr{x},t)+i\hat{\pi}\left( \vtr{x},t \right) \right)=\ldots \hat{a}_k e^{-i\omega_k t}
		\end{dmath}
		\begin{dmath}[]
			\hiderel{\Rightarrow} \hat{a}_k=\int_{}^{}\rd^3 \vtr{x}\, e^{ikx}\left( \omega_k\hat{\phi}+i\hat{\pi} \right)
		\end{dmath}
		\begin{dmath}[]
			\hat{a}_{k}^{\dagger}
			=\int_{}^{}\rd^3 x\, e^{-i\vtr{k}\vtr{x}}\left( \omega_{k}\hat{\phi}-i\hat{\pi} \right)
		\end{dmath}
		\begin{dsuspend}
			check consistency:
		\end{dsuspend}
		\begin{dmath}[]
			\comm{\hat{a}_k}{\hat{a}_{k'}^{\dagger}}
			=\int_{}^{}\rd^3 \vtr{x}\int_{}^{}\rd^3 \vtr{y}\, 
			e^{i\omega_k t-i\vtr{k}\vtr{x}}e^{-i\omega_{k'}t+i\vtr{k}'\vtr{x}}\comm{\omega_k\hat{\phi}+i\hat{\pi}}{\omega_{k'}\hat{\phi}\pm i\hat{\pi}}
		\end{dmath}
		\begin{dsuspend}
			where
		\end{dsuspend}
		\begin{dmath}[]
			\comm{\omega_k\hat{\phi}+i\hat{\pi}}{\omega_k\hat{\phi}\pm i\hat{\pi}}=\left( \omega_k\mp \omega_{k'} \right)\delta\left( \vtr{x}-\vtr{y} \right)
		\end{dmath}
		\begin{dmath}[]
			\hiderel{\leadsto}\comm{\hat{a}_k}{\hat{a}_{k'}^{\dagger}}
			=\int_{}^{}\rd^3 \vtr{x}\, e^{-i\vtr{x}\left( \vtr{k}-\vtr{k}' \right)}e^{i\left( \omega_{k}-\omega_{k'} \right)t}
			=\left( 2\pi \right)^3 2\omega_k\delta\left( \vtr{k}-\vtr{k}' \right)
		\end{dmath}
		\begin{dsuspend}
			where
		\end{dsuspend}
		\begin{dmath}[]
			\int_{}^{}\rd^3 \vtr{x} \,e^{-i\vtr{x}\left( \vtr{k}-\vtr{k}' \right)}=\left( 2\pi \right)^3 \delta\left( \vtr{k}-\vtr{k}' \right)
		\end{dmath}
		\begin{dmath}[]
			\hiderel{\leadsto} \hat{H}=\ldots
			=\frac{1}{2}\int_{}^{}\frac{\rd^3 \vtr{k}}{\left( 2\pi \right)^3}
			\frac{1}{2\omega_k}\omega_k\left( \hat{a}_{k}^{\dagger}\hat{a}_{k}+\underbrace{\hat{a}_k\hat{a}_{k}^{\dagger}}_{\hat{a}^{\dagger}\hat{a}_{k}+\sim\delta(0)} \right)
		\end{dmath}
		\begin{dsuspend}
			where $\delta(0)$ is infinite ground state energy but no absolute energy scale (only cae about energy differences)
		\end{dsuspend}
	\end{dgroup}
\end{proof}
nermal ordering: (anti) commute
all $\hat{a}^{\dagger}$ to the left of $\hat{a}$
\begin{dmath}[]
	\hat{H}\hiderel{:}=\int_{}^{}\frac{\rd^3 k}{\left( 2\pi \right)^3} \frac{1}{2\omega_k}\left( \hat{a}_{k}^{\dagger}\hat{a}_k \right)\omega_k\condition{subtracted $\mel{0}{H}{0}=\infty$}
\end{dmath}
\paragraph{Example 2: spin $\frac{1}{2}$ field}
\begin{dgroup}[]
	\begin{dmath}[]
		\mathcal{L}=\overline{\psi}(x)\left( i\cancel{\partial}-m \right)\psi(x)\condition{($\hbar=1$,$c=1$)}
	\end{dmath}
	\begin{dmath}[]
		\pdv{\mathcal{L}}{\psi}-\partial^{\mu}\pdv{\mathcal{L}}{\left( \partial^{\mu}\psi \right)}
		=0=-m\overline{\psi}-\partial^{\mu}\left( \overline{\psi}i\gamma_{\mu} \right)
		=\underbrace{\overline{\psi}\left( i\cancel{\partial}+m \right)}_{\mathclap{\text{adjoint Dirac equation}}}=0
	\end{dmath}
\end{dgroup}
Field momentum conjugate to $\psi$
\begin{dgroup}[]
	\begin{dmath}[]
		\pi\doteq \pdv{\mathcal{L}}{\dot{\phi}}
		=\overline{\psi}i\Gamma^{0}i\psi^{\dagger}
	\end{dmath}
	\begin{dsuspend}
		Hamiltonian
	\end{dsuspend}
	\begin{dmath}[]
		H=\int_{}^{}\rd^3 x\, \left( \pi \dot{\psi}-\mathcal{L} \right)
		=\int_{}^{}\rd^3 x\, i\psi^{\dagger}\dot{\psi}
	\end{dmath}
	\begin{dsuspend}
		add $\hat{}$ and impose
	\end{dsuspend}
	\begin{dmath}[]
		\acomm{\hat{\psi}_{\alpha}\left( \vtr{x},t \right)}{\hat{\psi}_{\beta}\left( \vtr{y},t \right)}
		=\acomm{\hat{\pi}_{\alpha}\left( \vtr{x},t \right)}{\hat{\pi}_{\beta}\left( \vtr{y},t \right)}
		=0
	\end{dmath}
	\begin{dmath}[]
		\acomm{\hat{\psi}_{\alpha}\left( \vtr{x},t \right)}{\hat{\pi}_{\beta}\left( \vtr{y},t \right)}
		=i\Delta_{\alpha\beta}\delta\left( \vtr{x}-\vtr{y} \right)
		\condition{$\alpha,\beta\in \left\{ 1,\cdots,4 \right\}$ spinor indices}
	\end{dmath}
\end{dgroup}
fermions $\Rightarrow$ use 
	\begin{dmath}[]
		\acomm{\cdot}{\cdot}=\comm{\cdot}{\cdot}_{+}
	\end{dmath}
		and not
	\begin{dmath}[]
		\comm{\cdot}{\cdot}=\comm{\cdot}{\cdot}_{-}
	\end{dmath}
field operators in momentum representaion 
\begin{dgroup}[]
	\begin{dmath}[]
		\hat{\psi}_{\alpha}=\int_{}^{}\frac{\rd^3 k}{\left( 2\pi \right)^3}\frac{1}{2\omega_k}\sum_{r=1}^{2}
		\left( \hat{b}\left( \vtr{k},r \right)U_{\alpha}\left( k,r \right)e^{-ikx}+\hat{d}^{\dagger}\left( k,r \right)V_{\alpha}(k,r)e^{ikx} \right)
	\end{dmath}
	\begin{dsuspend}
		where $\ds \int_{}^{}\frac{\rd^3 k}{\left( 2\pi \right)^3} \frac{1}{2\omega_k}$ is Lorentz invariant and $\sum_{r=1}^{2}$ from spin and $b^{\dagger}$ creates $E>0$ electrons and $d^{\dagger}$ creates a $E>0$ positron\\
		satisfies Dirac, since
	\end{dsuspend}
	\begin{dmath}[]
		\left( k-m \right)u=0
	\end{dmath}
	\begin{dmath}[]
		-k-m
	\end{dmath}v=0
\end{dgroup}
The anti commutation relations of the fields are consistent with
\begin{dgroup}[]
	\begin{dmath}[]
		\acomm{\hat{b}_{kr}}{\hat{b}_{k'r'}}
		=\acomm{\hat{d}_{kr}}{\hat{d}_{k'r'}^{\dagger}}
		=\left( 2\pi \right)^3 2\omega_k \delta_{rr'}\delta\left( \vtr{k}-\vtr{k}' \right)
	\end{dmath}
	\begin{dmath}[]
		\acomm{\hat{b}}{\hat{b}}
		=\acomm{\hat{b}^{\dagger}}{\hat{d}^{\dagger}}
		=\acomm{b}{d}=\ldots = 0
	\end{dmath}
\end{dgroup}
%Check:
%\begin{dgroup}[]
	%\begin{dmath}[]
		%\acomm{\hat{\psi}_{\alpha}}{\hat{\psi}_{\beta}^{\dagger}}
		%=\int_{}^{}\frac{\rd^3 k}{\left( 2\pi \right)^3}2\omega_{k}
		%\int_{}^{}\frac{\rd^3 k'}{\left( 2\pi \right)^32\omega_k'}\sum_{\text{?}}^{}
		%\left( \acomm{\hat{b}_{kr}}{\hat{b}_{k'r'}}U_{\alpha}\left( \vtr{k},r \right)U_{\beta}^{\dagger}\left( k',r' \right)e^{-ikx}e^{ik'y}+\acomm{\hat{d}_{kr}^{\dagger}}{\hat{d}_{k'r'}}V_{\alpha}\left( k,r \right)V_{\beta}^{\dagger}\left( k',r' \right)e^{ikr}e^{-ik'y} \right)
		%=\int_{}^{}\frac{\rd^3 k}{\left( 2\pi \right)^32\omega_k}\frac{1}{2\omega_k}\sum_{r}^{}\left( \underbrace{\left( U\left( k,r \right)\overline{U}\left( k,r \right)\gamma_0}_{\left( \left( k+m \right)\gamma_0 \right)_{\alpha\beta}} \right)_{\alpha\beta}e^{-ik\left( x-y \right)}-\left( \underbrace{U\left( k,r \right)\overline{U}\left( k,r \right)\gamma_0}_{\left( \left( -k+m \right)\gamma_0 \right)_{\alpha\beta}} \right)_{\alpha\beta}e^{ik\left( x-y \right)} \right)
		%=\int_{}^{}\frac{\rd^3 k}{\left( 2\pi \right)^3 2\omega_k}2\omega_k\sum_{r}^{}\left( \hat{b}_{kr}^{\dagger}\hat{b}_{kr}-\hat{d}_{kr}\hat{d}_{kr}^{\dagger} \right)
	%\end{dmath}
%\end{dgroup}
